lean/TtacExamples.lean
@@ -1,2 +1,3 @@
+import TtacExamples.BytemapVc
 import TtacExamples.Diamond
 import TtacExamples.DiamondVc
